proofs/fstar/extraction/Polytune.Data_types.fst
@@ -3,29 +3,14 @@ module Polytune.Data_types
 open Core
 open FStar.Mul
 
+/// The global key known only to a single party that is used to authenticate bits.
+type t_Delta = | Delta : u128 -> t_Delta
+
 /// A message authentication code held by a party together with an authenticated bit.
 type t_Mac = | Mac : u128 -> t_Mac
 
-[@@ FStar.Tactics.Typeclasses.tcinstance]
-let impl_2: Core.Ops.Bit.t_BitXor t_Mac t_Mac =
-  {
-    f_Output = t_Mac;
-    f_bitxor_pre = (fun (self: t_Mac) (rhs: t_Mac) -> true);
-    f_bitxor_post = (fun (self: t_Mac) (rhs: t_Mac) (out: t_Mac) -> true);
-    f_bitxor = fun (self: t_Mac) (rhs: t_Mac) -> Mac (self._0 ^. rhs._0) <: t_Mac
-  }
-
 /// A key used to authenticate (together with the [Delta] global key) a bit for the other party.
 type t_Key = | Key : u128 -> t_Key
-
-[@@ FStar.Tactics.Typeclasses.tcinstance]
-let impl_4: Core.Ops.Bit.t_BitXor t_Key t_Key =
-  {
-    f_Output = t_Key;
-    f_bitxor_pre = (fun (self: t_Key) (rhs: t_Key) -> true);
-    f_bitxor_post = (fun (self: t_Key) (rhs: t_Key) (out: t_Key) -> true);
-    f_bitxor = fun (self: t_Key) (rhs: t_Key) -> Key (self._0 ^. rhs._0) <: t_Key
-  }
 
 type t_Auth = | Auth : Alloc.Vec.t_Vec (t_Mac & t_Key) Alloc.Alloc.t_Global -> t_Auth
 
