proofs/fstar/extraction/Polytune.Faand.fst
@@ -6,8 +6,15 @@ open FStar.Mul
 let _ =
   (* This module has implicit dependencies, here we make them explicit. *)
   (* The implicit dependencies arise from typeclasses instances. *)
-  let open Polytune.Data_types in
+  let open Polytune.Channel in
+  let open Serde.De in
+  let open Serde.De.Impls in
+  let open Serde.Ser in
+  let open Serde.Ser.Impls in
   ()
+
+/// The statistical security parameter `RHO` used for cryptographic operations.
+let v_RHO: usize = mk_usize 40
 
 /// Errors occurring during preprocessing.
 type t_Error =
@@ -20,215 +27,1233 @@ type t_Error =
   | Error_EmptyMsg : t_Error
   | Error_InvalidLength : t_Error
   | Error_InconsistentBroadcast : t_Error
-  | Error_KOSConsistencyCheckFailed : t_Error
   | Error_ABitWrongMAC : t_Error
   | Error_AShareWrongMAC : t_Error
   | Error_LaANDXorNotZero : t_Error
   | Error_AANDWrongMAC : t_Error
   | Error_BeaverWrongMAC : t_Error
   | Error_InvalidHashLength : t_Error
+  | Error_OTError : Polytune.Swankyot.t_Error -> t_Error
 
-/// Combine two leaky ANDs into one non-leaky AND.
-let combine_two_leaky_ands (i n: usize) (x1 y1 z1 x2 z2: Polytune.Data_types.t_Share) (d: bool)
-    : Prims.Pure
-      (Core.Result.t_Result
-          (Polytune.Data_types.t_Share & Polytune.Data_types.t_Share & Polytune.Data_types.t_Share)
-          t_Error)
-      (requires
-        (Alloc.Vec.impl_1__len #(Polytune.Data_types.t_Mac & Polytune.Data_types.t_Key)
-            #Alloc.Alloc.t_Global
-            x1.Polytune.Data_types._1.Polytune.Data_types._0
-          <:
-          usize) >=.
-        n &&
-        (Alloc.Vec.impl_1__len #(Polytune.Data_types.t_Mac & Polytune.Data_types.t_Key)
-            #Alloc.Alloc.t_Global
-            x2.Polytune.Data_types._1.Polytune.Data_types._0
-          <:
-          usize) >=.
-        n &&
-        (Alloc.Vec.impl_1__len #(Polytune.Data_types.t_Mac & Polytune.Data_types.t_Key)
-            #Alloc.Alloc.t_Global
-            z1.Polytune.Data_types._1.Polytune.Data_types._0
-          <:
-          usize) >=.
-        n &&
-        (Alloc.Vec.impl_1__len #(Polytune.Data_types.t_Mac & Polytune.Data_types.t_Key)
-            #Alloc.Alloc.t_Global
-            z2.Polytune.Data_types._1.Polytune.Data_types._0
-          <:
-          usize) >=.
-        n)
-      (fun _ -> Prims.l_True) =
-  let xbit:bool = Core.Ops.Bit.f_bitxor x1.Polytune.Data_types._0 x2.Polytune.Data_types._0 in
-  let xauth:Polytune.Data_types.t_Auth =
-    Polytune.Data_types.Auth
-    (Alloc.Vec.from_elem #(Polytune.Data_types.t_Mac & Polytune.Data_types.t_Key)
-        ((Polytune.Data_types.Mac (mk_u128 0) <: Polytune.Data_types.t_Mac),
-          (Polytune.Data_types.Key (mk_u128 0) <: Polytune.Data_types.t_Key)
-          <:
-          (Polytune.Data_types.t_Mac & Polytune.Data_types.t_Key))
-        n)
+/// Represents a cryptographic commitment as a fixed-size 32-byte array (a BLAKE3 hash).
+type t_Commitment = | Commitment : t_Array u8 (mk_usize 32) -> t_Commitment
+
+[@@ FStar.Tactics.Typeclasses.tcinstance]
+assume
+val impl_3': Core.Fmt.t_Debug t_Commitment
+
+let impl_3 = impl_3'
+
+[@@ FStar.Tactics.Typeclasses.tcinstance]
+assume
+val e___impl': Serde.Ser.t_Serialize t_Commitment
+
+let e___impl = e___impl'
+
+[@@ FStar.Tactics.Typeclasses.tcinstance]
+assume
+val e_ee_1__impl': Serde.De.t_Deserialize t_Commitment
+
+let e_ee_1__impl = e_ee_1__impl'
+
+[@@ FStar.Tactics.Typeclasses.tcinstance]
+assume
+val impl_7': Core.Cmp.t_PartialEq t_Commitment t_Commitment
+
+let impl_7 = impl_7'
+
+/// Commits to a value using the BLAKE3 cryptographic hash function.
+/// This is not a general-purpose commitment scheme, the input value is assumed to have high entropy.
+assume
+val commit': value: t_Slice u8 -> t_Commitment
+
+let commit = commit'
+
+/// Verifies if a given value matches a previously generated commitment.
+/// This is not a general-purpose commitment scheme, the input value is assumed to have high entropy.
+assume
+val open_commitment': commitment: t_Commitment -> value: t_Slice u8 -> bool
+
+let open_commitment = open_commitment'
+
+/// Implements broadcast with abort based on Goldwasser and Lindell\'s protocol
+/// for all parties at once, where each party sends its vector to all others.
+/// The function returns the vector received and verified by broadcast.
+assume
+val broadcast':
+    #v_T: Type0 ->
+    #iimpl_951670863_: Type0 ->
+    {| i2: Core.Clone.t_Clone v_T |} ->
+    {| i3: Serde.Ser.t_Serialize v_T |} ->
+    {| i4: Serde.De.t_DeserializeOwned v_T |} ->
+    {| i5: Core.Fmt.t_Debug v_T |} ->
+    {| i6: Core.Cmp.t_PartialEq v_T v_T |} ->
+    {| i7: Polytune.Channel.t_Channel iimpl_951670863_ |} ->
+    channel: iimpl_951670863_ ->
+    i: usize ->
+    n: usize ->
+    phase: string ->
+    vec: t_Slice v_T ->
+    len: usize
+  -> (iimpl_951670863_ &
+      Core.Result.t_Result
+        (Alloc.Vec.t_Vec (Alloc.Vec.t_Vec v_T Alloc.Alloc.t_Global) Alloc.Alloc.t_Global) t_Error)
+
+let broadcast
+      (#v_T #iimpl_951670863_: Type0)
+      (#[FStar.Tactics.Typeclasses.tcresolve ()] i2: Core.Clone.t_Clone v_T)
+      (#[FStar.Tactics.Typeclasses.tcresolve ()] i3: Serde.Ser.t_Serialize v_T)
+      (#[FStar.Tactics.Typeclasses.tcresolve ()] i4: Serde.De.t_DeserializeOwned v_T)
+      (#[FStar.Tactics.Typeclasses.tcresolve ()] i5: Core.Fmt.t_Debug v_T)
+      (#[FStar.Tactics.Typeclasses.tcresolve ()] i6: Core.Cmp.t_PartialEq v_T v_T)
+      (#[FStar.Tactics.Typeclasses.tcresolve ()] i7: Polytune.Channel.t_Channel iimpl_951670863_)
+     = broadcast' #v_T #iimpl_951670863_ #i2 #i3 #i4 #i5 #i6 #i7
+
+/// Protocol PI_aBit^n that performs F_aBit^n from the paper
+/// [Global-Scale Secure Multiparty Computation](https://dl.acm.org/doi/pdf/10.1145/3133956.3133979).
+/// This function implements a secure multi-party computation protocol to generate a random
+/// bit-string and the corresponding keys and MACs (the latter are sent to the other parties),
+/// i.e., shares of random authenticated bits.
+/// The two main steps of the protocol are running two-party oblivious transfers (OTs) for
+/// each pair of parties and then checking the validity of the MACs and keys by checking the XOR
+/// of a linear combination of the bits, keys and the MACs and then removing 2 * RHO objects,
+/// where RHO is the statistical security parameter.
+assume
+val fabitn':
+    #iimpl_951670863_: Type0 ->
+    {| i1: Polytune.Channel.t_Channel iimpl_951670863_ |} ->
+    channel: iimpl_951670863_ ->
+    delta: Polytune.Data_types.t_Delta ->
+    i: usize ->
+    n: usize ->
+    l: usize ->
+    shared_two_by_two: Alloc.Vec.t_Vec Rand_chacha.Chacha.t_ChaCha20Rng Alloc.Alloc.t_Global
+  -> (iimpl_951670863_ &
+      Core.Result.t_Result
+        (Alloc.Vec.t_Vec Polytune.Data_types.t_Share Alloc.Alloc.t_Global &
+          Rand_chacha.Chacha.t_ChaCha20Rng) t_Error)
+
+let fabitn
+      (#iimpl_951670863_: Type0)
+      (#[FStar.Tactics.Typeclasses.tcresolve ()] i1: Polytune.Channel.t_Channel iimpl_951670863_)
+     = fabitn' #iimpl_951670863_ #i1
+
+/// Protocol PI_aShare that performs F_aShare from the paper
+/// [Global-Scale Secure Multiparty Computation](https://dl.acm.org/doi/pdf/10.1145/3133956.3133979).
+/// This protocol allows parties to generate and distribute authenticated random shares securely.
+/// It consists of the following steps:
+/// 1. **Random Bit String Generation**: Each party picks a random bit string of a specified length.
+/// 2. **Autenticated Bit Generation**: The parties generate random authenticated bit shares.
+/// 3. **Commitment and Verification**:
+///    - The parties compute commitments based on a subset of their shares and broadcast these to ensure consistency.
+///    - They then verify these commitments by performing decommitments and checking the validity of the
+///      MACs against the commitments.
+/// 4. **Return Shares**: Finally, the function returns the first `l` authenticated bit shares.
+let fashare
+      (#iimpl_951670863_: Type0)
+      (#[FStar.Tactics.Typeclasses.tcresolve ()] i1: Polytune.Channel.t_Channel iimpl_951670863_)
+      (channel: iimpl_951670863_)
+      (delta: Polytune.Data_types.t_Delta)
+      (i n l: usize)
+      (shared_two_by_two: Alloc.Vec.t_Vec Rand_chacha.Chacha.t_ChaCha20Rng Alloc.Alloc.t_Global)
+    : (iimpl_951670863_ &
+      Core.Result.t_Result
+        (Alloc.Vec.t_Vec Polytune.Data_types.t_Share Alloc.Alloc.t_Global &
+          Rand_chacha.Chacha.t_ChaCha20Rng) t_Error) =
+  let tmp0, out:(iimpl_951670863_ &
+    Core.Result.t_Result
+      (Alloc.Vec.t_Vec Polytune.Data_types.t_Share Alloc.Alloc.t_Global &
+        Rand_chacha.Chacha.t_ChaCha20Rng) t_Error) =
+    fabitn #iimpl_951670863_ channel delta i n (l +! v_RHO <: usize) shared_two_by_two
+  in
+  let channel:iimpl_951670863_ = tmp0 in
+  match
+    out
     <:
-    Polytune.Data_types.t_Auth
-  in
-  let xauth:Polytune.Data_types.t_Auth =
-    Rust_primitives.Hax.Folds.fold_range (mk_usize 0)
-      n
-      (fun xauth k ->
-          let xauth:Polytune.Data_types.t_Auth = xauth in
-          let k:usize = k in
-          (Alloc.Vec.impl_1__len #(Polytune.Data_types.t_Mac & Polytune.Data_types.t_Key)
-              #Alloc.Alloc.t_Global
-              xauth.Polytune.Data_types._0
-            <:
-            usize) =.
-          n
+    Core.Result.t_Result
+      (Alloc.Vec.t_Vec Polytune.Data_types.t_Share Alloc.Alloc.t_Global &
+        Rand_chacha.Chacha.t_ChaCha20Rng) t_Error
+  with
+  | Core.Result.Result_Ok (xishares, multi_shared_rand) ->
+    let d0:Alloc.Vec.t_Vec u128 Alloc.Alloc.t_Global =
+      Alloc.Vec.from_elem #u128 (mk_u128 0) v_RHO
+    in
+    let d1:Alloc.Vec.t_Vec u128 Alloc.Alloc.t_Global =
+      Alloc.Vec.from_elem #u128 (mk_u128 0) v_RHO
+    in
+    let c0_c1_cm:Alloc.Vec.t_Vec (t_Commitment & t_Commitment & t_Commitment) Alloc.Alloc.t_Global =
+      Alloc.Vec.impl__with_capacity #(t_Commitment & t_Commitment & t_Commitment) v_RHO
+    in
+    let dmvec:Alloc.Vec.t_Vec (Alloc.Vec.t_Vec u8 Alloc.Alloc.t_Global) Alloc.Alloc.t_Global =
+      Alloc.Vec.impl__with_capacity #(Alloc.Vec.t_Vec u8 Alloc.Alloc.t_Global) v_RHO
+    in
+    let c0_c1_cm, d0, d1, dmvec:(Alloc.Vec.t_Vec (t_Commitment & t_Commitment & t_Commitment)
+        Alloc.Alloc.t_Global &
+      Alloc.Vec.t_Vec u128 Alloc.Alloc.t_Global &
+      Alloc.Vec.t_Vec u128 Alloc.Alloc.t_Global &
+      Alloc.Vec.t_Vec (Alloc.Vec.t_Vec u8 Alloc.Alloc.t_Global) Alloc.Alloc.t_Global) =
+      Rust_primitives.Hax.Folds.fold_range (mk_usize 0)
+        v_RHO
+        (fun temp_0_ temp_1_ ->
+            let c0_c1_cm, d0, d1, dmvec:(Alloc.Vec.t_Vec
+                (t_Commitment & t_Commitment & t_Commitment) Alloc.Alloc.t_Global &
+              Alloc.Vec.t_Vec u128 Alloc.Alloc.t_Global &
+              Alloc.Vec.t_Vec u128 Alloc.Alloc.t_Global &
+              Alloc.Vec.t_Vec (Alloc.Vec.t_Vec u8 Alloc.Alloc.t_Global) Alloc.Alloc.t_Global) =
+              temp_0_
+            in
+            let _:usize = temp_1_ in
+            true)
+        (c0_c1_cm, d0, d1, dmvec
           <:
-          bool)
-      xauth
-      (fun xauth k ->
-          let xauth:Polytune.Data_types.t_Auth = xauth in
-          let k:usize = k in
-          if k =. i <: bool
-          then xauth
-          else
-            let mk_x1, ki_x1:(Polytune.Data_types.t_Mac & Polytune.Data_types.t_Key) =
-              x1.Polytune.Data_types._1.Polytune.Data_types._0.[ k ]
+          (Alloc.Vec.t_Vec (t_Commitment & t_Commitment & t_Commitment) Alloc.Alloc.t_Global &
+            Alloc.Vec.t_Vec u128 Alloc.Alloc.t_Global &
+            Alloc.Vec.t_Vec u128 Alloc.Alloc.t_Global &
+            Alloc.Vec.t_Vec (Alloc.Vec.t_Vec u8 Alloc.Alloc.t_Global) Alloc.Alloc.t_Global))
+        (fun temp_0_ r ->
+            let c0_c1_cm, d0, d1, dmvec:(Alloc.Vec.t_Vec
+                (t_Commitment & t_Commitment & t_Commitment) Alloc.Alloc.t_Global &
+              Alloc.Vec.t_Vec u128 Alloc.Alloc.t_Global &
+              Alloc.Vec.t_Vec u128 Alloc.Alloc.t_Global &
+              Alloc.Vec.t_Vec (Alloc.Vec.t_Vec u8 Alloc.Alloc.t_Global) Alloc.Alloc.t_Global) =
+              temp_0_
             in
-            let mk_x2, ki_x2:(Polytune.Data_types.t_Mac & Polytune.Data_types.t_Key) =
-              x2.Polytune.Data_types._1.Polytune.Data_types._0.[ k ]
+            let r:usize = r in
+            let xishare:Polytune.Data_types.t_Share = xishares.[ l +! r <: usize ] in
+            let dm:Alloc.Vec.t_Vec u8 Alloc.Alloc.t_Global =
+              Alloc.Vec.impl__with_capacity #u8 (n *! mk_usize 16 <: usize)
             in
-            {
-              xauth with
-              Polytune.Data_types._0
-              =
-              Rust_primitives.Hax.Monomorphized_update_at.update_at_usize xauth
-                  .Polytune.Data_types._0
-                k
-                ((Core.Ops.Bit.f_bitxor #Polytune.Data_types.t_Mac
-                      #Polytune.Data_types.t_Mac
-                      #FStar.Tactics.Typeclasses.solve
-                      mk_x1
-                      mk_x2
-                    <:
-                    Polytune.Data_types.t_Mac),
-                  (Core.Ops.Bit.f_bitxor #Polytune.Data_types.t_Key
-                      #Polytune.Data_types.t_Key
-                      #FStar.Tactics.Typeclasses.solve
-                      ki_x1
-                      ki_x2
-                    <:
-                    Polytune.Data_types.t_Key)
+            let dm:Alloc.Vec.t_Vec u8 Alloc.Alloc.t_Global =
+              Alloc.Vec.impl_1__push #u8
+                #Alloc.Alloc.t_Global
+                dm
+                (cast (xishare.Polytune.Data_types._0 <: bool) <: u8)
+            in
+            let d0, dm:(Alloc.Vec.t_Vec u128 Alloc.Alloc.t_Global &
+              Alloc.Vec.t_Vec u8 Alloc.Alloc.t_Global) =
+              Rust_primitives.Hax.Folds.fold_range (mk_usize 0)
+                n
+                (fun temp_0_ temp_1_ ->
+                    let d0, dm:(Alloc.Vec.t_Vec u128 Alloc.Alloc.t_Global &
+                      Alloc.Vec.t_Vec u8 Alloc.Alloc.t_Global) =
+                      temp_0_
+                    in
+                    let _:usize = temp_1_ in
+                    true)
+                (d0, dm
                   <:
-                  (Polytune.Data_types.t_Mac & Polytune.Data_types.t_Key))
-            }
+                  (Alloc.Vec.t_Vec u128 Alloc.Alloc.t_Global &
+                    Alloc.Vec.t_Vec u8 Alloc.Alloc.t_Global))
+                (fun temp_0_ k ->
+                    let d0, dm:(Alloc.Vec.t_Vec u128 Alloc.Alloc.t_Global &
+                      Alloc.Vec.t_Vec u8 Alloc.Alloc.t_Global) =
+                      temp_0_
+                    in
+                    let k:usize = k in
+                    if k =. i <: bool
+                    then
+                      d0, dm
+                      <:
+                      (Alloc.Vec.t_Vec u128 Alloc.Alloc.t_Global &
+                        Alloc.Vec.t_Vec u8 Alloc.Alloc.t_Global)
+                    else
+                      let mac, key:(Polytune.Data_types.t_Mac & Polytune.Data_types.t_Key) =
+                        xishare.Polytune.Data_types._1.Polytune.Data_types._0.[ k ]
+                      in
+                      let d0:Alloc.Vec.t_Vec u128 Alloc.Alloc.t_Global =
+                        Rust_primitives.Hax.Monomorphized_update_at.update_at_usize d0
+                          r
+                          (key.Polytune.Data_types._0 ^. (d0.[ r ] <: u128) <: u128)
+                      in
+                      let dm:Alloc.Vec.t_Vec u8 Alloc.Alloc.t_Global =
+                        Core.Iter.Traits.Collect.f_extend #(Alloc.Vec.t_Vec u8 Alloc.Alloc.t_Global)
+                          #u8
+                          #FStar.Tactics.Typeclasses.solve
+                          #(t_Array u8 (mk_usize 16))
+                          dm
+                          (Core.Num.impl_u128__to_be_bytes mac.Polytune.Data_types._0
+                            <:
+                            t_Array u8 (mk_usize 16))
+                      in
+                      d0, dm
+                      <:
+                      (Alloc.Vec.t_Vec u128 Alloc.Alloc.t_Global &
+                        Alloc.Vec.t_Vec u8 Alloc.Alloc.t_Global))
+            in
+            let d1:Alloc.Vec.t_Vec u128 Alloc.Alloc.t_Global =
+              Rust_primitives.Hax.Monomorphized_update_at.update_at_usize d1
+                r
+                ((d0.[ r ] <: u128) ^. delta.Polytune.Data_types._0 <: u128)
+            in
+            let c0:t_Commitment =
+              commit (Core.Num.impl_u128__to_be_bytes (d0.[ r ] <: u128) <: t_Slice u8)
+            in
+            let c1:t_Commitment =
+              commit (Core.Num.impl_u128__to_be_bytes (d1.[ r ] <: u128) <: t_Slice u8)
+            in
+            let cm:t_Commitment =
+              commit (Core.Ops.Deref.f_deref #(Alloc.Vec.t_Vec u8 Alloc.Alloc.t_Global)
+                    #FStar.Tactics.Typeclasses.solve
+                    dm
+                  <:
+                  t_Slice u8)
+            in
+            let c0_c1_cm:Alloc.Vec.t_Vec (t_Commitment & t_Commitment & t_Commitment)
+              Alloc.Alloc.t_Global =
+              Alloc.Vec.impl_1__push #(t_Commitment & t_Commitment & t_Commitment)
+                #Alloc.Alloc.t_Global
+                c0_c1_cm
+                (c0, c1, cm <: (t_Commitment & t_Commitment & t_Commitment))
+            in
+            let dmvec:Alloc.Vec.t_Vec (Alloc.Vec.t_Vec u8 Alloc.Alloc.t_Global) Alloc.Alloc.t_Global
+            =
+              Alloc.Vec.impl_1__push #(Alloc.Vec.t_Vec u8 Alloc.Alloc.t_Global)
+                #Alloc.Alloc.t_Global
+                dmvec
+                dm
+            in
+            c0_c1_cm, d0, d1, dmvec
             <:
-            Polytune.Data_types.t_Auth)
-  in
-  let xshare:Polytune.Data_types.t_Share =
-    Polytune.Data_types.Share xbit xauth <: Polytune.Data_types.t_Share
-  in
-  let zbit:bool =
-    Core.Ops.Bit.f_bitxor (Core.Ops.Bit.f_bitxor z1.Polytune.Data_types._0 z2.Polytune.Data_types._0
+            (Alloc.Vec.t_Vec (t_Commitment & t_Commitment & t_Commitment) Alloc.Alloc.t_Global &
+              Alloc.Vec.t_Vec u128 Alloc.Alloc.t_Global &
+              Alloc.Vec.t_Vec u128 Alloc.Alloc.t_Global &
+              Alloc.Vec.t_Vec (Alloc.Vec.t_Vec u8 Alloc.Alloc.t_Global) Alloc.Alloc.t_Global))
+    in
+    let tmp0, out:(iimpl_951670863_ &
+      Core.Result.t_Result
+        (Alloc.Vec.t_Vec
+            (Alloc.Vec.t_Vec (t_Commitment & t_Commitment & t_Commitment) Alloc.Alloc.t_Global)
+            Alloc.Alloc.t_Global) t_Error) =
+      broadcast #(t_Commitment & t_Commitment & t_Commitment)
+        #iimpl_951670863_
+        channel
+        i
+        n
+        "fashare comm"
+        (Core.Ops.Deref.f_deref #(Alloc.Vec.t_Vec (t_Commitment & t_Commitment & t_Commitment)
+                Alloc.Alloc.t_Global)
+            #FStar.Tactics.Typeclasses.solve
+            c0_c1_cm
+          <:
+          t_Slice (t_Commitment & t_Commitment & t_Commitment))
+        v_RHO
+    in
+    let channel:iimpl_951670863_ = tmp0 in
+    (match
+        out
         <:
-        bool)
-      (Core.Ops.Bit.f_bitand d x2.Polytune.Data_types._0 <: bool)
-  in
-  let zauth:Polytune.Data_types.t_Auth =
-    Polytune.Data_types.Auth
-    (Alloc.Vec.from_elem #(Polytune.Data_types.t_Mac & Polytune.Data_types.t_Key)
-        ((Polytune.Data_types.Mac (mk_u128 0) <: Polytune.Data_types.t_Mac),
-          (Polytune.Data_types.Key (mk_u128 0) <: Polytune.Data_types.t_Key)
-          <:
-          (Polytune.Data_types.t_Mac & Polytune.Data_types.t_Key))
-        n)
-    <:
-    Polytune.Data_types.t_Auth
-  in
-  let zauth:Polytune.Data_types.t_Auth =
-    Rust_primitives.Hax.Folds.fold_range (mk_usize 0)
-      n
-      (fun zauth k ->
-          let zauth:Polytune.Data_types.t_Auth = zauth in
-          let k:usize = k in
-          (Alloc.Vec.impl_1__len #(Polytune.Data_types.t_Mac & Polytune.Data_types.t_Key)
-              #Alloc.Alloc.t_Global
-              zauth.Polytune.Data_types._0
+        Core.Result.t_Result
+          (Alloc.Vec.t_Vec
+              (Alloc.Vec.t_Vec (t_Commitment & t_Commitment & t_Commitment) Alloc.Alloc.t_Global)
+              Alloc.Alloc.t_Global) t_Error
+      with
+      | Core.Result.Result_Ok c0_c1_cm_k ->
+        let c0_c1_cm_k:Alloc.Vec.t_Vec
+          (Alloc.Vec.t_Vec (t_Commitment & t_Commitment & t_Commitment) Alloc.Alloc.t_Global)
+          Alloc.Alloc.t_Global =
+          Rust_primitives.Hax.Monomorphized_update_at.update_at_usize c0_c1_cm_k i c0_c1_cm
+        in
+        let tmp0, out:(iimpl_951670863_ &
+          Core.Result.t_Result
+            (Alloc.Vec.t_Vec
+                (Alloc.Vec.t_Vec (Alloc.Vec.t_Vec u8 Alloc.Alloc.t_Global) Alloc.Alloc.t_Global)
+                Alloc.Alloc.t_Global) t_Error) =
+          broadcast #(Alloc.Vec.t_Vec u8 Alloc.Alloc.t_Global)
+            #iimpl_951670863_
+            channel
+            i
+            n
+            "fashare ver"
+            (Core.Ops.Deref.f_deref #(Alloc.Vec.t_Vec (Alloc.Vec.t_Vec u8 Alloc.Alloc.t_Global)
+                    Alloc.Alloc.t_Global)
+                #FStar.Tactics.Typeclasses.solve
+                dmvec
+              <:
+              t_Slice (Alloc.Vec.t_Vec u8 Alloc.Alloc.t_Global))
+            v_RHO
+        in
+        let channel:iimpl_951670863_ = tmp0 in
+        (match
+            out
             <:
-            usize) =.
-          n
-          <:
-          bool)
-      zauth
-      (fun zauth k ->
-          let zauth:Polytune.Data_types.t_Auth = zauth in
-          let k:usize = k in
-          if k =. i <: bool
-          then zauth
-          else
-            let mk_z1, ki_z1:(Polytune.Data_types.t_Mac & Polytune.Data_types.t_Key) =
-              z1.Polytune.Data_types._1.Polytune.Data_types._0.[ k ]
+            Core.Result.t_Result
+              (Alloc.Vec.t_Vec
+                  (Alloc.Vec.t_Vec (Alloc.Vec.t_Vec u8 Alloc.Alloc.t_Global) Alloc.Alloc.t_Global)
+                  Alloc.Alloc.t_Global) t_Error
+          with
+          | Core.Result.Result_Ok dm_k ->
+            let dm_k:Alloc.Vec.t_Vec
+              (Alloc.Vec.t_Vec (Alloc.Vec.t_Vec u8 Alloc.Alloc.t_Global) Alloc.Alloc.t_Global)
+              Alloc.Alloc.t_Global =
+              Rust_primitives.Hax.Monomorphized_update_at.update_at_usize dm_k i dmvec
             in
-            let mk_z2, ki_z2:(Polytune.Data_types.t_Mac & Polytune.Data_types.t_Key) =
-              z2.Polytune.Data_types._1.Polytune.Data_types._0.[ k ]
+            let (bi: t_Array bool (mk_usize 40)):t_Array bool (mk_usize 40) =
+              Rust_primitives.Hax.repeat false (mk_usize 40)
             in
-            let mk_x2, ki_x2:(Polytune.Data_types.t_Mac & Polytune.Data_types.t_Key) =
-              x2.Polytune.Data_types._1.Polytune.Data_types._0.[ k ]
+            let di_bi:Alloc.Vec.t_Vec u128 Alloc.Alloc.t_Global =
+              Alloc.Vec.from_elem #u128 (mk_u128 0) v_RHO
             in
-            {
-              zauth with
-              Polytune.Data_types._0
-              =
-              Rust_primitives.Hax.Monomorphized_update_at.update_at_usize zauth
-                  .Polytune.Data_types._0
-                k
-                ((Core.Ops.Bit.f_bitxor #Polytune.Data_types.t_Mac
-                      #Polytune.Data_types.t_Mac
-                      #FStar.Tactics.Typeclasses.solve
-                      (Core.Ops.Bit.f_bitxor #Polytune.Data_types.t_Mac
-                          #Polytune.Data_types.t_Mac
-                          #FStar.Tactics.Typeclasses.solve
-                          mk_z1
-                          mk_z2
+            (match
+                Rust_primitives.Hax.Folds.fold_range_return (mk_usize 0)
+                  v_RHO
+                  (fun di_bi temp_1_ ->
+                      let di_bi:Alloc.Vec.t_Vec u128 Alloc.Alloc.t_Global = di_bi in
+                      let _:usize = temp_1_ in
+                      true)
+                  di_bi
+                  (fun di_bi r ->
+                      let di_bi:Alloc.Vec.t_Vec u128 Alloc.Alloc.t_Global = di_bi in
+                      let r:usize = r in
+                      match
+                        Rust_primitives.Hax.Folds.fold_range_return (mk_usize 0)
+                          n
+                          (fun temp_0_ temp_1_ ->
+                              let _:Prims.unit = temp_0_ in
+                              let _:usize = temp_1_ in
+                              true)
+                          ()
+                          (fun temp_0_ k ->
+                              let _:Prims.unit = temp_0_ in
+                              let k:usize = k in
+                              if k =. i <: bool
+                              then
+                                Core.Ops.Control_flow.ControlFlow_Continue (() <: Prims.unit)
+                                <:
+                                Core.Ops.Control_flow.t_ControlFlow
+                                  (Core.Ops.Control_flow.t_ControlFlow
+                                      (iimpl_951670863_ &
+                                        Core.Result.t_Result
+                                          (Alloc.Vec.t_Vec Polytune.Data_types.t_Share
+                                              Alloc.Alloc.t_Global &
+                                            Rand_chacha.Chacha.t_ChaCha20Rng) t_Error)
+                                      (Prims.unit & Prims.unit)) Prims.unit
+                              else
+                                if
+                                  (((dm_k.[ k ]
+                                        <:
+                                        Alloc.Vec.t_Vec (Alloc.Vec.t_Vec u8 Alloc.Alloc.t_Global)
+                                          Alloc.Alloc.t_Global).[ r ]
+                                      <:
+                                      Alloc.Vec.t_Vec u8 Alloc.Alloc.t_Global).[ mk_usize 0 ]
+                                    <:
+                                    u8) >.
+                                  mk_u8 1
+                                  <:
+                                  bool
+                                then
+                                  Core.Ops.Control_flow.ControlFlow_Break
+                                  (Core.Ops.Control_flow.ControlFlow_Break
+                                    (channel,
+                                      (Core.Result.Result_Err (Error_InvalidBitValue <: t_Error)
+                                        <:
+                                        Core.Result.t_Result
+                                          (Alloc.Vec.t_Vec Polytune.Data_types.t_Share
+                                              Alloc.Alloc.t_Global &
+                                            Rand_chacha.Chacha.t_ChaCha20Rng) t_Error)
+                                      <:
+                                      (iimpl_951670863_ &
+                                        Core.Result.t_Result
+                                          (Alloc.Vec.t_Vec Polytune.Data_types.t_Share
+                                              Alloc.Alloc.t_Global &
+                                            Rand_chacha.Chacha.t_ChaCha20Rng) t_Error))
+                                    <:
+                                    Core.Ops.Control_flow.t_ControlFlow
+                                      (iimpl_951670863_ &
+                                        Core.Result.t_Result
+                                          (Alloc.Vec.t_Vec Polytune.Data_types.t_Share
+                                              Alloc.Alloc.t_Global &
+                                            Rand_chacha.Chacha.t_ChaCha20Rng) t_Error)
+                                      (Prims.unit & Prims.unit))
+                                  <:
+                                  Core.Ops.Control_flow.t_ControlFlow
+                                    (Core.Ops.Control_flow.t_ControlFlow
+                                        (iimpl_951670863_ &
+                                          Core.Result.t_Result
+                                            (Alloc.Vec.t_Vec Polytune.Data_types.t_Share
+                                                Alloc.Alloc.t_Global &
+                                              Rand_chacha.Chacha.t_ChaCha20Rng) t_Error)
+                                        (Prims.unit & Prims.unit)) Prims.unit
+                                else
+                                  let cond:bool =
+                                    (((dm_k.[ k ]
+                                          <:
+                                          Alloc.Vec.t_Vec (Alloc.Vec.t_Vec u8 Alloc.Alloc.t_Global)
+                                            Alloc.Alloc.t_Global).[ r ]
+                                        <:
+                                        Alloc.Vec.t_Vec u8 Alloc.Alloc.t_Global).[ mk_usize 0 ]
+                                      <:
+                                      u8) <>.
+                                    mk_u8 0
+                                  in
+                                  Core.Ops.Control_flow.ControlFlow_Continue ()
+                                  <:
+                                  Core.Ops.Control_flow.t_ControlFlow
+                                    (Core.Ops.Control_flow.t_ControlFlow
+                                        (iimpl_951670863_ &
+                                          Core.Result.t_Result
+                                            (Alloc.Vec.t_Vec Polytune.Data_types.t_Share
+                                                Alloc.Alloc.t_Global &
+                                              Rand_chacha.Chacha.t_ChaCha20Rng) t_Error)
+                                        (Prims.unit & Prims.unit)) Prims.unit)
                         <:
-                        Polytune.Data_types.t_Mac)
-                      (Polytune.Data_types.Mac
-                        ((cast (d <: bool) <: u128) *! mk_x2.Polytune.Data_types._0 <: u128)
+                        Core.Ops.Control_flow.t_ControlFlow
+                          (iimpl_951670863_ &
+                            Core.Result.t_Result
+                              (Alloc.Vec.t_Vec Polytune.Data_types.t_Share Alloc.Alloc.t_Global &
+                                Rand_chacha.Chacha.t_ChaCha20Rng) t_Error) Prims.unit
+                      with
+                      | Core.Ops.Control_flow.ControlFlow_Break ret ->
+                        Core.Ops.Control_flow.ControlFlow_Break
+                        (Core.Ops.Control_flow.ControlFlow_Break ret
+                          <:
+                          Core.Ops.Control_flow.t_ControlFlow
+                            (iimpl_951670863_ &
+                              Core.Result.t_Result
+                                (Alloc.Vec.t_Vec Polytune.Data_types.t_Share Alloc.Alloc.t_Global &
+                                  Rand_chacha.Chacha.t_ChaCha20Rng) t_Error)
+                            (Prims.unit & Alloc.Vec.t_Vec u128 Alloc.Alloc.t_Global))
                         <:
-                        Polytune.Data_types.t_Mac)
-                    <:
-                    Polytune.Data_types.t_Mac),
-                  (Core.Ops.Bit.f_bitxor #Polytune.Data_types.t_Key
-                      #Polytune.Data_types.t_Key
-                      #FStar.Tactics.Typeclasses.solve
-                      (Core.Ops.Bit.f_bitxor #Polytune.Data_types.t_Key
-                          #Polytune.Data_types.t_Key
-                          #FStar.Tactics.Typeclasses.solve
-                          ki_z1
-                          ki_z2
+                        Core.Ops.Control_flow.t_ControlFlow
+                          (Core.Ops.Control_flow.t_ControlFlow
+                              (iimpl_951670863_ &
+                                Core.Result.t_Result
+                                  (Alloc.Vec.t_Vec Polytune.Data_types.t_Share Alloc.Alloc.t_Global &
+                                    Rand_chacha.Chacha.t_ChaCha20Rng) t_Error)
+                              (Prims.unit & Alloc.Vec.t_Vec u128 Alloc.Alloc.t_Global))
+                          (Alloc.Vec.t_Vec u128 Alloc.Alloc.t_Global)
+                      | Core.Ops.Control_flow.ControlFlow_Continue _ ->
+                        Core.Ops.Control_flow.ControlFlow_Continue
+                        (Rust_primitives.Hax.Monomorphized_update_at.update_at_usize di_bi
+                            r
+                            (if bi.[ r ] <: bool then d1.[ r ] <: u128 else d0.[ r ] <: u128)
+                          <:
+                          Alloc.Vec.t_Vec u128 Alloc.Alloc.t_Global)
                         <:
-                        Polytune.Data_types.t_Key)
-                      (Polytune.Data_types.Key
-                        ((cast (d <: bool) <: u128) *! ki_x2.Polytune.Data_types._0 <: u128)
-                        <:
-                        Polytune.Data_types.t_Key)
-                    <:
-                    Polytune.Data_types.t_Key)
+                        Core.Ops.Control_flow.t_ControlFlow
+                          (Core.Ops.Control_flow.t_ControlFlow
+                              (iimpl_951670863_ &
+                                Core.Result.t_Result
+                                  (Alloc.Vec.t_Vec Polytune.Data_types.t_Share Alloc.Alloc.t_Global &
+                                    Rand_chacha.Chacha.t_ChaCha20Rng) t_Error)
+                              (Prims.unit & Alloc.Vec.t_Vec u128 Alloc.Alloc.t_Global))
+                          (Alloc.Vec.t_Vec u128 Alloc.Alloc.t_Global))
+                <:
+                Core.Ops.Control_flow.t_ControlFlow
+                  (iimpl_951670863_ &
+                    Core.Result.t_Result
+                      (Alloc.Vec.t_Vec Polytune.Data_types.t_Share Alloc.Alloc.t_Global &
+                        Rand_chacha.Chacha.t_ChaCha20Rng) t_Error)
+                  (Alloc.Vec.t_Vec u128 Alloc.Alloc.t_Global)
+              with
+              | Core.Ops.Control_flow.ControlFlow_Break ret -> ret
+              | Core.Ops.Control_flow.ControlFlow_Continue di_bi ->
+                let tmp0, out:(iimpl_951670863_ &
+                  Core.Result.t_Result
+                    (Alloc.Vec.t_Vec (Alloc.Vec.t_Vec u128 Alloc.Alloc.t_Global)
+                        Alloc.Alloc.t_Global) t_Error) =
+                  broadcast #u128
+                    #iimpl_951670863_
+                    channel
+                    i
+                    n
+                    "fashare di_bi"
+                    (Core.Ops.Deref.f_deref #(Alloc.Vec.t_Vec u128 Alloc.Alloc.t_Global)
+                        #FStar.Tactics.Typeclasses.solve
+                        di_bi
+                      <:
+                      t_Slice u128)
+                    v_RHO
+                in
+                let channel:iimpl_951670863_ = tmp0 in
+                match
+                  out
                   <:
-                  (Polytune.Data_types.t_Mac & Polytune.Data_types.t_Key))
-            }
+                  Core.Result.t_Result
+                    (Alloc.Vec.t_Vec (Alloc.Vec.t_Vec u128 Alloc.Alloc.t_Global)
+                        Alloc.Alloc.t_Global) t_Error
+                with
+                | Core.Result.Result_Ok di_bi_k ->
+                  let xor_xk_macs:Alloc.Vec.t_Vec (Alloc.Vec.t_Vec u128 Alloc.Alloc.t_Global)
+                    Alloc.Alloc.t_Global =
+                    Alloc.Vec.from_elem #(Alloc.Vec.t_Vec u128 Alloc.Alloc.t_Global)
+                      (Alloc.Vec.from_elem #u128 (mk_u128 0) v_RHO
+                        <:
+                        Alloc.Vec.t_Vec u128 Alloc.Alloc.t_Global)
+                      n
+                  in
+                  (match
+                      Rust_primitives.Hax.Folds.fold_range_return (mk_usize 0)
+                        v_RHO
+                        (fun xor_xk_macs temp_1_ ->
+                            let xor_xk_macs:Alloc.Vec.t_Vec
+                              (Alloc.Vec.t_Vec u128 Alloc.Alloc.t_Global) Alloc.Alloc.t_Global =
+                              xor_xk_macs
+                            in
+                            let _:usize = temp_1_ in
+                            true)
+                        xor_xk_macs
+                        (fun xor_xk_macs r ->
+                            let xor_xk_macs:Alloc.Vec.t_Vec
+                              (Alloc.Vec.t_Vec u128 Alloc.Alloc.t_Global) Alloc.Alloc.t_Global =
+                              xor_xk_macs
+                            in
+                            let r:usize = r in
+                            match
+                              Rust_primitives.Hax.Folds.fold_return (Core.Iter.Traits.Collect.f_into_iter
+                                    #(Core.Iter.Adapters.Take.t_Take
+                                      (Core.Iter.Adapters.Enumerate.t_Enumerate
+                                        (Core.Slice.Iter.t_Iter
+                                          (Alloc.Vec.t_Vec (Alloc.Vec.t_Vec u8 Alloc.Alloc.t_Global)
+                                              Alloc.Alloc.t_Global))))
+                                    #FStar.Tactics.Typeclasses.solve
+                                    (Core.Iter.Traits.Iterator.f_take #(Core.Iter.Adapters.Enumerate.t_Enumerate
+                                          (Core.Slice.Iter.t_Iter
+                                            (Alloc.Vec.t_Vec
+                                                (Alloc.Vec.t_Vec u8 Alloc.Alloc.t_Global)
+                                                Alloc.Alloc.t_Global)))
+                                        #FStar.Tactics.Typeclasses.solve
+                                        (Core.Iter.Traits.Iterator.f_enumerate #(Core.Slice.Iter.t_Iter
+                                              (Alloc.Vec.t_Vec
+                                                  (Alloc.Vec.t_Vec u8 Alloc.Alloc.t_Global)
+                                                  Alloc.Alloc.t_Global))
+                                            #FStar.Tactics.Typeclasses.solve
+                                            (Core.Slice.impl__iter #(Alloc.Vec.t_Vec
+                                                    (Alloc.Vec.t_Vec u8 Alloc.Alloc.t_Global)
+                                                    Alloc.Alloc.t_Global)
+                                                (Core.Ops.Deref.f_deref #(Alloc.Vec.t_Vec
+                                                        (Alloc.Vec.t_Vec
+                                                            (Alloc.Vec.t_Vec u8 Alloc.Alloc.t_Global
+                                                            ) Alloc.Alloc.t_Global)
+                                                        Alloc.Alloc.t_Global)
+                                                    #FStar.Tactics.Typeclasses.solve
+                                                    dm_k
+                                                  <:
+                                                  t_Slice
+                                                  (Alloc.Vec.t_Vec
+                                                      (Alloc.Vec.t_Vec u8 Alloc.Alloc.t_Global)
+                                                      Alloc.Alloc.t_Global))
+                                              <:
+                                              Core.Slice.Iter.t_Iter
+                                              (Alloc.Vec.t_Vec
+                                                  (Alloc.Vec.t_Vec u8 Alloc.Alloc.t_Global)
+                                                  Alloc.Alloc.t_Global))
+                                          <:
+                                          Core.Iter.Adapters.Enumerate.t_Enumerate
+                                          (Core.Slice.Iter.t_Iter
+                                            (Alloc.Vec.t_Vec
+                                                (Alloc.Vec.t_Vec u8 Alloc.Alloc.t_Global)
+                                                Alloc.Alloc.t_Global)))
+                                        n
+                                      <:
+                                      Core.Iter.Adapters.Take.t_Take
+                                      (Core.Iter.Adapters.Enumerate.t_Enumerate
+                                        (Core.Slice.Iter.t_Iter
+                                          (Alloc.Vec.t_Vec (Alloc.Vec.t_Vec u8 Alloc.Alloc.t_Global)
+                                              Alloc.Alloc.t_Global))))
+                                  <:
+                                  Core.Iter.Adapters.Take.t_Take
+                                  (Core.Iter.Adapters.Enumerate.t_Enumerate
+                                    (Core.Slice.Iter.t_Iter
+                                      (Alloc.Vec.t_Vec (Alloc.Vec.t_Vec u8 Alloc.Alloc.t_Global)
+                                          Alloc.Alloc.t_Global))))
+                                xor_xk_macs
+                                (fun xor_xk_macs temp_1_ ->
+                                    let xor_xk_macs:Alloc.Vec.t_Vec
+                                      (Alloc.Vec.t_Vec u128 Alloc.Alloc.t_Global)
+                                      Alloc.Alloc.t_Global =
+                                      xor_xk_macs
+                                    in
+                                    let k, dmv:(usize &
+                                      Alloc.Vec.t_Vec (Alloc.Vec.t_Vec u8 Alloc.Alloc.t_Global)
+                                        Alloc.Alloc.t_Global) =
+                                      temp_1_
+                                    in
+                                    match
+                                      Rust_primitives.Hax.Folds.fold_range_return (mk_usize 0)
+                                        n
+                                        (fun xor_xk_macs temp_1_ ->
+                                            let xor_xk_macs:Alloc.Vec.t_Vec
+                                              (Alloc.Vec.t_Vec u128 Alloc.Alloc.t_Global)
+                                              Alloc.Alloc.t_Global =
+                                              xor_xk_macs
+                                            in
+                                            let _:usize = temp_1_ in
+                                            true)
+                                        xor_xk_macs
+                                        (fun xor_xk_macs kk ->
+                                            let xor_xk_macs:Alloc.Vec.t_Vec
+                                              (Alloc.Vec.t_Vec u128 Alloc.Alloc.t_Global)
+                                              Alloc.Alloc.t_Global =
+                                              xor_xk_macs
+                                            in
+                                            let kk:usize = kk in
+                                            if kk =. k <: bool
+                                            then
+                                              Core.Ops.Control_flow.ControlFlow_Continue xor_xk_macs
+                                              <:
+                                              Core.Ops.Control_flow.t_ControlFlow
+                                                (Core.Ops.Control_flow.t_ControlFlow
+                                                    (iimpl_951670863_ &
+                                                      Core.Result.t_Result
+                                                        (Alloc.Vec.t_Vec Polytune.Data_types.t_Share
+                                                            Alloc.Alloc.t_Global &
+                                                          Rand_chacha.Chacha.t_ChaCha20Rng) t_Error)
+                                                    (Prims.unit &
+                                                      Alloc.Vec.t_Vec
+                                                        (Alloc.Vec.t_Vec u128 Alloc.Alloc.t_Global)
+                                                        Alloc.Alloc.t_Global))
+                                                (Alloc.Vec.t_Vec
+                                                    (Alloc.Vec.t_Vec u128 Alloc.Alloc.t_Global)
+                                                    Alloc.Alloc.t_Global)
+                                            else
+                                              if
+                                                Alloc.Vec.impl_1__is_empty #(Alloc.Vec.t_Vec u8
+                                                      Alloc.Alloc.t_Global)
+                                                  #Alloc.Alloc.t_Global
+                                                  dmv
+                                                <:
+                                                bool
+                                              then
+                                                Core.Ops.Control_flow.ControlFlow_Break
+                                                (Core.Ops.Control_flow.ControlFlow_Break
+                                                  (channel,
+                                                    (Core.Result.Result_Err
+                                                      (Error_EmptyVector <: t_Error)
+                                                      <:
+                                                      Core.Result.t_Result
+                                                        (Alloc.Vec.t_Vec Polytune.Data_types.t_Share
+                                                            Alloc.Alloc.t_Global &
+                                                          Rand_chacha.Chacha.t_ChaCha20Rng) t_Error)
+                                                    <:
+                                                    (iimpl_951670863_ &
+                                                      Core.Result.t_Result
+                                                        (Alloc.Vec.t_Vec Polytune.Data_types.t_Share
+                                                            Alloc.Alloc.t_Global &
+                                                          Rand_chacha.Chacha.t_ChaCha20Rng) t_Error)
+                                                  )
+                                                  <:
+                                                  Core.Ops.Control_flow.t_ControlFlow
+                                                    (iimpl_951670863_ &
+                                                      Core.Result.t_Result
+                                                        (Alloc.Vec.t_Vec Polytune.Data_types.t_Share
+                                                            Alloc.Alloc.t_Global &
+                                                          Rand_chacha.Chacha.t_ChaCha20Rng) t_Error)
+                                                    (Prims.unit &
+                                                      Alloc.Vec.t_Vec
+                                                        (Alloc.Vec.t_Vec u128 Alloc.Alloc.t_Global)
+                                                        Alloc.Alloc.t_Global))
+                                                <:
+                                                Core.Ops.Control_flow.t_ControlFlow
+                                                  (Core.Ops.Control_flow.t_ControlFlow
+                                                      (iimpl_951670863_ &
+                                                        Core.Result.t_Result
+                                                          (Alloc.Vec.t_Vec
+                                                              Polytune.Data_types.t_Share
+                                                              Alloc.Alloc.t_Global &
+                                                            Rand_chacha.Chacha.t_ChaCha20Rng)
+                                                          t_Error)
+                                                      (Prims.unit &
+                                                        Alloc.Vec.t_Vec
+                                                          (Alloc.Vec.t_Vec u128 Alloc.Alloc.t_Global
+                                                          ) Alloc.Alloc.t_Global))
+                                                  (Alloc.Vec.t_Vec
+                                                      (Alloc.Vec.t_Vec u128 Alloc.Alloc.t_Global)
+                                                      Alloc.Alloc.t_Global)
+                                              else
+                                                let dm:Alloc.Vec.t_Vec u8 Alloc.Alloc.t_Global =
+                                                  dmv.[ r ]
+                                                in
+                                                let start:usize =
+                                                  if kk >. k
+                                                  then
+                                                    mk_usize 1 +!
+                                                    ((kk -! mk_usize 1 <: usize) *! mk_usize 16
+                                                      <:
+                                                      usize)
+                                                  else mk_usize 1 +! (kk *! mk_usize 16 <: usize)
+                                                in
+                                                let v_end:usize = start +! mk_usize 16 in
+                                                match
+                                                  Core.Result.impl__map #(t_Array u8 (mk_usize 16))
+                                                    #Core.Array.t_TryFromSliceError
+                                                    #u128
+                                                    (Core.Convert.f_try_into #(t_Slice u8)
+                                                        #(t_Array u8 (mk_usize 16))
+                                                        #FStar.Tactics.Typeclasses.solve
+                                                        (dm.[ {
+                                                              Core.Ops.Range.f_start = start;
+                                                              Core.Ops.Range.f_end = v_end
+                                                            }
+                                                            <:
+                                                            Core.Ops.Range.t_Range usize ]
+                                                          <:
+                                                          t_Slice u8)
+                                                      <:
+                                                      Core.Result.t_Result
+                                                        (t_Array u8 (mk_usize 16))
+                                                        Core.Array.t_TryFromSliceError)
+                                                    Core.Num.impl_u128__from_be_bytes
+                                                  <:
+                                                  Core.Result.t_Result u128
+                                                    Core.Array.t_TryFromSliceError
+                                                with
+                                                | Core.Result.Result_Ok mac ->
+                                                  let xor_xk_macs:Alloc.Vec.t_Vec
+                                                    (Alloc.Vec.t_Vec u128 Alloc.Alloc.t_Global)
+                                                    Alloc.Alloc.t_Global =
+                                                    Rust_primitives.Hax.Monomorphized_update_at.update_at_usize
+                                                      xor_xk_macs
+                                                      kk
+                                                      (Rust_primitives.Hax.Monomorphized_update_at.update_at_usize
+                                                          (xor_xk_macs.[ kk ]
+                                                            <:
+                                                            Alloc.Vec.t_Vec u128
+                                                              Alloc.Alloc.t_Global)
+                                                          r
+                                                          (mac ^.
+                                                            ((xor_xk_macs.[ kk ]
+                                                                <:
+                                                                Alloc.Vec.t_Vec u128
+                                                                  Alloc.Alloc.t_Global).[ r ]
+                                                              <:
+                                                              u128)
+                                                            <:
+                                                            u128)
+                                                        <:
+                                                        Alloc.Vec.t_Vec u128 Alloc.Alloc.t_Global)
+                                                  in
+                                                  Core.Ops.Control_flow.ControlFlow_Continue
+                                                  xor_xk_macs
+                                                  <:
+                                                  Core.Ops.Control_flow.t_ControlFlow
+                                                    (Core.Ops.Control_flow.t_ControlFlow
+                                                        (iimpl_951670863_ &
+                                                          Core.Result.t_Result
+                                                            (Alloc.Vec.t_Vec
+                                                                Polytune.Data_types.t_Share
+                                                                Alloc.Alloc.t_Global &
+                                                              Rand_chacha.Chacha.t_ChaCha20Rng)
+                                                            t_Error)
+                                                        (Prims.unit &
+                                                          Alloc.Vec.t_Vec
+                                                            (Alloc.Vec.t_Vec u128
+                                                                Alloc.Alloc.t_Global)
+                                                            Alloc.Alloc.t_Global))
+                                                    (Alloc.Vec.t_Vec
+                                                        (Alloc.Vec.t_Vec u128 Alloc.Alloc.t_Global)
+                                                        Alloc.Alloc.t_Global)
+                                                | _ ->
+                                                  Core.Ops.Control_flow.ControlFlow_Break
+                                                  (Core.Ops.Control_flow.ControlFlow_Break
+                                                    (channel,
+                                                      (Core.Result.Result_Err
+                                                        (Error_ConversionErr <: t_Error)
+                                                        <:
+                                                        Core.Result.t_Result
+                                                          (Alloc.Vec.t_Vec
+                                                              Polytune.Data_types.t_Share
+                                                              Alloc.Alloc.t_Global &
+                                                            Rand_chacha.Chacha.t_ChaCha20Rng)
+                                                          t_Error)
+                                                      <:
+                                                      (iimpl_951670863_ &
+                                                        Core.Result.t_Result
+                                                          (Alloc.Vec.t_Vec
+                                                              Polytune.Data_types.t_Share
+                                                              Alloc.Alloc.t_Global &
+                                                            Rand_chacha.Chacha.t_ChaCha20Rng)
+                                                          t_Error))
+                                                    <:
+                                                    Core.Ops.Control_flow.t_ControlFlow
+                                                      (iimpl_951670863_ &
+                                                        Core.Result.t_Result
+                                                          (Alloc.Vec.t_Vec
+                                                              Polytune.Data_types.t_Share
+                                                              Alloc.Alloc.t_Global &
+                                                            Rand_chacha.Chacha.t_ChaCha20Rng)
+                                                          t_Error)
+                                                      (Prims.unit &
+                                                        Alloc.Vec.t_Vec
+                                                          (Alloc.Vec.t_Vec u128 Alloc.Alloc.t_Global
+                                                          ) Alloc.Alloc.t_Global))
+                                                  <:
+                                                  Core.Ops.Control_flow.t_ControlFlow
+                                                    (Core.Ops.Control_flow.t_ControlFlow
+                                                        (iimpl_951670863_ &
+                                                          Core.Result.t_Result
+                                                            (Alloc.Vec.t_Vec
+                                                                Polytune.Data_types.t_Share
+                                                                Alloc.Alloc.t_Global &
+                                                              Rand_chacha.Chacha.t_ChaCha20Rng)
+                                                            t_Error)
+                                                        (Prims.unit &
+                                                          Alloc.Vec.t_Vec
+                                                            (Alloc.Vec.t_Vec u128
+                                                                Alloc.Alloc.t_Global)
+                                                            Alloc.Alloc.t_Global))
+                                                    (Alloc.Vec.t_Vec
+                                                        (Alloc.Vec.t_Vec u128 Alloc.Alloc.t_Global)
+                                                        Alloc.Alloc.t_Global))
+                                      <:
+                                      Core.Ops.Control_flow.t_ControlFlow
+                                        (iimpl_951670863_ &
+                                          Core.Result.t_Result
+                                            (Alloc.Vec.t_Vec Polytune.Data_types.t_Share
+                                                Alloc.Alloc.t_Global &
+                                              Rand_chacha.Chacha.t_ChaCha20Rng) t_Error)
+                                        (Alloc.Vec.t_Vec (Alloc.Vec.t_Vec u128 Alloc.Alloc.t_Global)
+                                            Alloc.Alloc.t_Global)
+                                    with
+                                    | Core.Ops.Control_flow.ControlFlow_Break ret ->
+                                      Core.Ops.Control_flow.ControlFlow_Break
+                                      (Core.Ops.Control_flow.ControlFlow_Break ret
+                                        <:
+                                        Core.Ops.Control_flow.t_ControlFlow
+                                          (iimpl_951670863_ &
+                                            Core.Result.t_Result
+                                              (Alloc.Vec.t_Vec Polytune.Data_types.t_Share
+                                                  Alloc.Alloc.t_Global &
+                                                Rand_chacha.Chacha.t_ChaCha20Rng) t_Error)
+                                          (Prims.unit &
+                                            Alloc.Vec.t_Vec
+                                              (Alloc.Vec.t_Vec u128 Alloc.Alloc.t_Global)
+                                              Alloc.Alloc.t_Global))
+                                      <:
+                                      Core.Ops.Control_flow.t_ControlFlow
+                                        (Core.Ops.Control_flow.t_ControlFlow
+                                            (iimpl_951670863_ &
+                                              Core.Result.t_Result
+                                                (Alloc.Vec.t_Vec Polytune.Data_types.t_Share
+                                                    Alloc.Alloc.t_Global &
+                                                  Rand_chacha.Chacha.t_ChaCha20Rng) t_Error)
+                                            (Prims.unit &
+                                              Alloc.Vec.t_Vec
+                                                (Alloc.Vec.t_Vec u128 Alloc.Alloc.t_Global)
+                                                Alloc.Alloc.t_Global))
+                                        (Alloc.Vec.t_Vec (Alloc.Vec.t_Vec u128 Alloc.Alloc.t_Global)
+                                            Alloc.Alloc.t_Global)
+                                    | Core.Ops.Control_flow.ControlFlow_Continue loop_res ->
+                                      Core.Ops.Control_flow.ControlFlow_Continue loop_res
+                                      <:
+                                      Core.Ops.Control_flow.t_ControlFlow
+                                        (Core.Ops.Control_flow.t_ControlFlow
+                                            (iimpl_951670863_ &
+                                              Core.Result.t_Result
+                                                (Alloc.Vec.t_Vec Polytune.Data_types.t_Share
+                                                    Alloc.Alloc.t_Global &
+                                                  Rand_chacha.Chacha.t_ChaCha20Rng) t_Error)
+                                            (Prims.unit &
+                                              Alloc.Vec.t_Vec
+                                                (Alloc.Vec.t_Vec u128 Alloc.Alloc.t_Global)
+                                                Alloc.Alloc.t_Global))
+                                        (Alloc.Vec.t_Vec (Alloc.Vec.t_Vec u128 Alloc.Alloc.t_Global)
+                                            Alloc.Alloc.t_Global))
+                              <:
+                              Core.Ops.Control_flow.t_ControlFlow
+                                (iimpl_951670863_ &
+                                  Core.Result.t_Result
+                                    (Alloc.Vec.t_Vec Polytune.Data_types.t_Share
+                                        Alloc.Alloc.t_Global &
+                                      Rand_chacha.Chacha.t_ChaCha20Rng) t_Error)
+                                (Alloc.Vec.t_Vec (Alloc.Vec.t_Vec u128 Alloc.Alloc.t_Global)
+                                    Alloc.Alloc.t_Global)
+                            with
+                            | Core.Ops.Control_flow.ControlFlow_Break ret ->
+                              Core.Ops.Control_flow.ControlFlow_Break
+                              (Core.Ops.Control_flow.ControlFlow_Break ret
+                                <:
+                                Core.Ops.Control_flow.t_ControlFlow
+                                  (iimpl_951670863_ &
+                                    Core.Result.t_Result
+                                      (Alloc.Vec.t_Vec Polytune.Data_types.t_Share
+                                          Alloc.Alloc.t_Global &
+                                        Rand_chacha.Chacha.t_ChaCha20Rng) t_Error)
+                                  (Prims.unit &
+                                    Alloc.Vec.t_Vec (Alloc.Vec.t_Vec u128 Alloc.Alloc.t_Global)
+                                      Alloc.Alloc.t_Global))
+                              <:
+                              Core.Ops.Control_flow.t_ControlFlow
+                                (Core.Ops.Control_flow.t_ControlFlow
+                                    (iimpl_951670863_ &
+                                      Core.Result.t_Result
+                                        (Alloc.Vec.t_Vec Polytune.Data_types.t_Share
+                                            Alloc.Alloc.t_Global &
+                                          Rand_chacha.Chacha.t_ChaCha20Rng) t_Error)
+                                    (Prims.unit &
+                                      Alloc.Vec.t_Vec (Alloc.Vec.t_Vec u128 Alloc.Alloc.t_Global)
+                                        Alloc.Alloc.t_Global))
+                                (Alloc.Vec.t_Vec (Alloc.Vec.t_Vec u128 Alloc.Alloc.t_Global)
+                                    Alloc.Alloc.t_Global)
+                            | Core.Ops.Control_flow.ControlFlow_Continue xor_xk_macs ->
+                              match
+                                Rust_primitives.Hax.Folds.fold_range_return (mk_usize 0)
+                                  n
+                                  (fun temp_0_ temp_1_ ->
+                                      let _:Prims.unit = temp_0_ in
+                                      let _:usize = temp_1_ in
+                                      true)
+                                  ()
+                                  (fun temp_0_ k ->
+                                      let _:Prims.unit = temp_0_ in
+                                      let k:usize = k in
+                                      if k =. i <: bool
+                                      then
+                                        Core.Ops.Control_flow.ControlFlow_Continue
+                                        (() <: Prims.unit)
+                                        <:
+                                        Core.Ops.Control_flow.t_ControlFlow
+                                          (Core.Ops.Control_flow.t_ControlFlow
+                                              (iimpl_951670863_ &
+                                                Core.Result.t_Result
+                                                  (Alloc.Vec.t_Vec Polytune.Data_types.t_Share
+                                                      Alloc.Alloc.t_Global &
+                                                    Rand_chacha.Chacha.t_ChaCha20Rng) t_Error)
+                                              (Prims.unit & Prims.unit)) Prims.unit
+                                      else
+                                        let d_bj:t_Array u8 (mk_usize 16) =
+                                          Core.Num.impl_u128__to_be_bytes ((di_bi_k.[ k ]
+                                                <:
+                                                Alloc.Vec.t_Vec u128 Alloc.Alloc.t_Global).[ r ]
+                                              <:
+                                              u128)
+                                        in
+                                        let commitments:(t_Commitment & t_Commitment & t_Commitment)
+                                        =
+                                          (c0_c1_cm_k.[ k ]
+                                            <:
+                                            Alloc.Vec.t_Vec
+                                              (t_Commitment & t_Commitment & t_Commitment)
+                                              Alloc.Alloc.t_Global).[ r ]
+                                        in
+                                        if
+                                          ~.(open_commitment commitments._1 (d_bj <: t_Slice u8)
+                                            <:
+                                            bool) &&
+                                          ~.(open_commitment commitments._2 (d_bj <: t_Slice u8)
+                                            <:
+                                            bool)
+                                        then
+                                          Core.Ops.Control_flow.ControlFlow_Break
+                                          (Core.Ops.Control_flow.ControlFlow_Break
+                                            (channel,
+                                              (Core.Result.Result_Err
+                                                (Error_CommitmentCouldNotBeOpened <: t_Error)
+                                                <:
+                                                Core.Result.t_Result
+                                                  (Alloc.Vec.t_Vec Polytune.Data_types.t_Share
+                                                      Alloc.Alloc.t_Global &
+                                                    Rand_chacha.Chacha.t_ChaCha20Rng) t_Error)
+                                              <:
+                                              (iimpl_951670863_ &
+                                                Core.Result.t_Result
+                                                  (Alloc.Vec.t_Vec Polytune.Data_types.t_Share
+                                                      Alloc.Alloc.t_Global &
+                                                    Rand_chacha.Chacha.t_ChaCha20Rng) t_Error))
+                                            <:
+                                            Core.Ops.Control_flow.t_ControlFlow
+                                              (iimpl_951670863_ &
+                                                Core.Result.t_Result
+                                                  (Alloc.Vec.t_Vec Polytune.Data_types.t_Share
+                                                      Alloc.Alloc.t_Global &
+                                                    Rand_chacha.Chacha.t_ChaCha20Rng) t_Error)
+                                              (Prims.unit & Prims.unit))
+                                          <:
+                                          Core.Ops.Control_flow.t_ControlFlow
+                                            (Core.Ops.Control_flow.t_ControlFlow
+                                                (iimpl_951670863_ &
+                                                  Core.Result.t_Result
+                                                    (Alloc.Vec.t_Vec Polytune.Data_types.t_Share
+                                                        Alloc.Alloc.t_Global &
+                                                      Rand_chacha.Chacha.t_ChaCha20Rng) t_Error)
+                                                (Prims.unit & Prims.unit)) Prims.unit
+                                        else
+                                          if
+                                            ((xor_xk_macs.[ k ]
+                                                <:
+                                                Alloc.Vec.t_Vec u128 Alloc.Alloc.t_Global).[ r ]
+                                              <:
+                                              u128) <>.
+                                            ((di_bi_k.[ k ]
+                                                <:
+                                                Alloc.Vec.t_Vec u128 Alloc.Alloc.t_Global).[ r ]
+                                              <:
+                                              u128)
+                                          then
+                                            Core.Ops.Control_flow.ControlFlow_Break
+                                            (Core.Ops.Control_flow.ControlFlow_Break
+                                              (channel,
+                                                (Core.Result.Result_Err
+                                                  (Error_AShareWrongMAC <: t_Error)
+                                                  <:
+                                                  Core.Result.t_Result
+                                                    (Alloc.Vec.t_Vec Polytune.Data_types.t_Share
+                                                        Alloc.Alloc.t_Global &
+                                                      Rand_chacha.Chacha.t_ChaCha20Rng) t_Error)
+                                                <:
+                                                (iimpl_951670863_ &
+                                                  Core.Result.t_Result
+                                                    (Alloc.Vec.t_Vec Polytune.Data_types.t_Share
+                                                        Alloc.Alloc.t_Global &
+                                                      Rand_chacha.Chacha.t_ChaCha20Rng) t_Error))
+                                              <:
+                                              Core.Ops.Control_flow.t_ControlFlow
+                                                (iimpl_951670863_ &
+                                                  Core.Result.t_Result
+                                                    (Alloc.Vec.t_Vec Polytune.Data_types.t_Share
+                                                        Alloc.Alloc.t_Global &
+                                                      Rand_chacha.Chacha.t_ChaCha20Rng) t_Error)
+                                                (Prims.unit & Prims.unit))
+                                            <:
+                                            Core.Ops.Control_flow.t_ControlFlow
+                                              (Core.Ops.Control_flow.t_ControlFlow
+                                                  (iimpl_951670863_ &
+                                                    Core.Result.t_Result
+                                                      (Alloc.Vec.t_Vec Polytune.Data_types.t_Share
+                                                          Alloc.Alloc.t_Global &
+                                                        Rand_chacha.Chacha.t_ChaCha20Rng) t_Error)
+                                                  (Prims.unit & Prims.unit)) Prims.unit
+                                          else
+                                            Core.Ops.Control_flow.ControlFlow_Continue ()
+                                            <:
+                                            Core.Ops.Control_flow.t_ControlFlow
+                                              (Core.Ops.Control_flow.t_ControlFlow
+                                                  (iimpl_951670863_ &
+                                                    Core.Result.t_Result
+                                                      (Alloc.Vec.t_Vec Polytune.Data_types.t_Share
+                                                          Alloc.Alloc.t_Global &
+                                                        Rand_chacha.Chacha.t_ChaCha20Rng) t_Error)
+                                                  (Prims.unit & Prims.unit)) Prims.unit)
+                                <:
+                                Core.Ops.Control_flow.t_ControlFlow
+                                  (iimpl_951670863_ &
+                                    Core.Result.t_Result
+                                      (Alloc.Vec.t_Vec Polytune.Data_types.t_Share
+                                          Alloc.Alloc.t_Global &
+                                        Rand_chacha.Chacha.t_ChaCha20Rng) t_Error) Prims.unit
+                              with
+                              | Core.Ops.Control_flow.ControlFlow_Break ret ->
+                                Core.Ops.Control_flow.ControlFlow_Break
+                                (Core.Ops.Control_flow.ControlFlow_Break ret
+                                  <:
+                                  Core.Ops.Control_flow.t_ControlFlow
+                                    (iimpl_951670863_ &
+                                      Core.Result.t_Result
+                                        (Alloc.Vec.t_Vec Polytune.Data_types.t_Share
+                                            Alloc.Alloc.t_Global &
+                                          Rand_chacha.Chacha.t_ChaCha20Rng) t_Error)
+                                    (Prims.unit &
+                                      Alloc.Vec.t_Vec (Alloc.Vec.t_Vec u128 Alloc.Alloc.t_Global)
+                                        Alloc.Alloc.t_Global))
+                                <:
+                                Core.Ops.Control_flow.t_ControlFlow
+                                  (Core.Ops.Control_flow.t_ControlFlow
+                                      (iimpl_951670863_ &
+                                        Core.Result.t_Result
+                                          (Alloc.Vec.t_Vec Polytune.Data_types.t_Share
+                                              Alloc.Alloc.t_Global &
+                                            Rand_chacha.Chacha.t_ChaCha20Rng) t_Error)
+                                      (Prims.unit &
+                                        Alloc.Vec.t_Vec (Alloc.Vec.t_Vec u128 Alloc.Alloc.t_Global)
+                                          Alloc.Alloc.t_Global))
+                                  (Alloc.Vec.t_Vec (Alloc.Vec.t_Vec u128 Alloc.Alloc.t_Global)
+                                      Alloc.Alloc.t_Global)
+                              | Core.Ops.Control_flow.ControlFlow_Continue () ->
+                                Core.Ops.Control_flow.ControlFlow_Continue xor_xk_macs
+                                <:
+                                Core.Ops.Control_flow.t_ControlFlow
+                                  (Core.Ops.Control_flow.t_ControlFlow
+                                      (iimpl_951670863_ &
+                                        Core.Result.t_Result
+                                          (Alloc.Vec.t_Vec Polytune.Data_types.t_Share
+                                              Alloc.Alloc.t_Global &
+                                            Rand_chacha.Chacha.t_ChaCha20Rng) t_Error)
+                                      (Prims.unit &
+                                        Alloc.Vec.t_Vec (Alloc.Vec.t_Vec u128 Alloc.Alloc.t_Global)
+                                          Alloc.Alloc.t_Global))
+                                  (Alloc.Vec.t_Vec (Alloc.Vec.t_Vec u128 Alloc.Alloc.t_Global)
+                                      Alloc.Alloc.t_Global))
+                      <:
+                      Core.Ops.Control_flow.t_ControlFlow
+                        (iimpl_951670863_ &
+                          Core.Result.t_Result
+                            (Alloc.Vec.t_Vec Polytune.Data_types.t_Share Alloc.Alloc.t_Global &
+                              Rand_chacha.Chacha.t_ChaCha20Rng) t_Error)
+                        (Alloc.Vec.t_Vec (Alloc.Vec.t_Vec u128 Alloc.Alloc.t_Global)
+                            Alloc.Alloc.t_Global)
+                    with
+                    | Core.Ops.Control_flow.ControlFlow_Break ret -> ret
+                    | Core.Ops.Control_flow.ControlFlow_Continue xor_xk_macs ->
+                      let xishares:Alloc.Vec.t_Vec Polytune.Data_types.t_Share Alloc.Alloc.t_Global
+                      =
+                        Alloc.Vec.impl_1__truncate #Polytune.Data_types.t_Share
+                          #Alloc.Alloc.t_Global
+                          xishares
+                          l
+                      in
+                      let hax_temp_output:Core.Result.t_Result
+                        (Alloc.Vec.t_Vec Polytune.Data_types.t_Share Alloc.Alloc.t_Global &
+                          Rand_chacha.Chacha.t_ChaCha20Rng) t_Error =
+                        Core.Result.Result_Ok
+                        (xishares, multi_shared_rand
+                          <:
+                          (Alloc.Vec.t_Vec Polytune.Data_types.t_Share Alloc.Alloc.t_Global &
+                            Rand_chacha.Chacha.t_ChaCha20Rng))
+                        <:
+                        Core.Result.t_Result
+                          (Alloc.Vec.t_Vec Polytune.Data_types.t_Share Alloc.Alloc.t_Global &
+                            Rand_chacha.Chacha.t_ChaCha20Rng) t_Error
+                      in
+                      channel, hax_temp_output
+                      <:
+                      (iimpl_951670863_ &
+                        Core.Result.t_Result
+                          (Alloc.Vec.t_Vec Polytune.Data_types.t_Share Alloc.Alloc.t_Global &
+                            Rand_chacha.Chacha.t_ChaCha20Rng) t_Error))
+                | Core.Result.Result_Err err ->
+                  channel,
+                  (Core.Result.Result_Err err
+                    <:
+                    Core.Result.t_Result
+                      (Alloc.Vec.t_Vec Polytune.Data_types.t_Share Alloc.Alloc.t_Global &
+                        Rand_chacha.Chacha.t_ChaCha20Rng) t_Error)
+                  <:
+                  (iimpl_951670863_ &
+                    Core.Result.t_Result
+                      (Alloc.Vec.t_Vec Polytune.Data_types.t_Share Alloc.Alloc.t_Global &
+                        Rand_chacha.Chacha.t_ChaCha20Rng) t_Error))
+          | Core.Result.Result_Err err ->
+            channel,
+            (Core.Result.Result_Err err
+              <:
+              Core.Result.t_Result
+                (Alloc.Vec.t_Vec Polytune.Data_types.t_Share Alloc.Alloc.t_Global &
+                  Rand_chacha.Chacha.t_ChaCha20Rng) t_Error)
             <:
-            Polytune.Data_types.t_Auth)
-  in
-  let zshare:Polytune.Data_types.t_Share =
-    Polytune.Data_types.Share zbit zauth <: Polytune.Data_types.t_Share
-  in
-  Core.Result.Result_Ok
-  (xshare, y1, zshare
+            (iimpl_951670863_ &
+              Core.Result.t_Result
+                (Alloc.Vec.t_Vec Polytune.Data_types.t_Share Alloc.Alloc.t_Global &
+                  Rand_chacha.Chacha.t_ChaCha20Rng) t_Error))
+      | Core.Result.Result_Err err ->
+        channel,
+        (Core.Result.Result_Err err
+          <:
+          Core.Result.t_Result
+            (Alloc.Vec.t_Vec Polytune.Data_types.t_Share Alloc.Alloc.t_Global &
+              Rand_chacha.Chacha.t_ChaCha20Rng) t_Error)
+        <:
+        (iimpl_951670863_ &
+          Core.Result.t_Result
+            (Alloc.Vec.t_Vec Polytune.Data_types.t_Share Alloc.Alloc.t_Global &
+              Rand_chacha.Chacha.t_ChaCha20Rng) t_Error))
+  | Core.Result.Result_Err err ->
+    channel,
+    (Core.Result.Result_Err err
+      <:
+      Core.Result.t_Result
+        (Alloc.Vec.t_Vec Polytune.Data_types.t_Share Alloc.Alloc.t_Global &
+          Rand_chacha.Chacha.t_ChaCha20Rng) t_Error)
     <:
-    (Polytune.Data_types.t_Share & Polytune.Data_types.t_Share & Polytune.Data_types.t_Share))
-  <:
-  Core.Result.t_Result
-    (Polytune.Data_types.t_Share & Polytune.Data_types.t_Share & Polytune.Data_types.t_Share)
-    t_Error
+    (iimpl_951670863_ &
+      Core.Result.t_Result
+        (Alloc.Vec.t_Vec Polytune.Data_types.t_Share Alloc.Alloc.t_Global &
+          Rand_chacha.Chacha.t_ChaCha20Rng) t_Error)
