proofs/fstar/extraction/Polytune.Ot.fst
@@ -1,0 +1,47 @@
+module Polytune.Ot
+#set-options "--fuel 0 --ifuel 1 --z3rlimit 15"
+open Core
+open FStar.Mul
+
+let _ =
+  (* This module has implicit dependencies, here we make them explicit. *)
+  (* The implicit dependencies arise from typeclasses instances. *)
+  let open Polytune.Channel in
+  ()
+
+assume
+val kos_ot_sender':
+    #iimpl_951670863_: Type0 ->
+    {| i1: Polytune.Channel.t_Channel iimpl_951670863_ |} ->
+    channel: iimpl_951670863_ ->
+    delta: u128 ->
+    lprime: usize ->
+    p_to: usize ->
+    shared_rand: Rand_chacha.Chacha.t_ChaCha20Rng
+  -> (iimpl_951670863_ &
+      Core.Result.t_Result
+        (Alloc.Vec.t_Vec u128 Alloc.Alloc.t_Global & Rand_chacha.Chacha.t_ChaCha20Rng)
+        Polytune.Swankyot.t_Error)
+
+let kos_ot_sender
+      (#iimpl_951670863_: Type0)
+      (#[FStar.Tactics.Typeclasses.tcresolve ()] i1: Polytune.Channel.t_Channel iimpl_951670863_)
+     = kos_ot_sender' #iimpl_951670863_ #i1
+
+assume
+val kos_ot_receiver':
+    #iimpl_951670863_: Type0 ->
+    {| i1: Polytune.Channel.t_Channel iimpl_951670863_ |} ->
+    channel: iimpl_951670863_ ->
+    bs: t_Slice bool ->
+    p_to: usize ->
+    shared_rand: Rand_chacha.Chacha.t_ChaCha20Rng
+  -> (iimpl_951670863_ &
+      Core.Result.t_Result
+        (Alloc.Vec.t_Vec u128 Alloc.Alloc.t_Global & Rand_chacha.Chacha.t_ChaCha20Rng)
+        Polytune.Swankyot.t_Error)
+
+let kos_ot_receiver
+      (#iimpl_951670863_: Type0)
+      (#[FStar.Tactics.Typeclasses.tcresolve ()] i1: Polytune.Channel.t_Channel iimpl_951670863_)
+     = kos_ot_receiver' #iimpl_951670863_ #i1
