proofs/fstar/extraction/Rand.Distributions.Other.fst
@@ -1,0 +1,4 @@
+module Rand.Distributions.Other
+#set-options "--fuel 0 --ifuel 1 --z3rlimit 15"
+
+type t_ChaCha20Rng = ()
