proofs/fstar/extraction/Serde.Ser.fst
@@ -1,0 +1,7 @@
+module Serde.Ser
+#set-options "--fuel 0 --ifuel 1 --z3rlimit 15"
+
+class t_Serialize (t_Self:Type) = {
+  serialize: t_Self -> t_Self
+  }
+
